feat: use ⇒ instead of : to match agda book more

Plfl/Lambda.lean
@@ -26,9 +26,9 @@ inductive Term where
 deriving BEq, DecidableEq, Repr
 
 namespace Term
-  notation:50 "ƛ " v " : " d => lam v d
-  notation:50 " μ " v " : " d => mu v d
-  notation:max "𝟘? " e " [zero: " o " |succ " n " : " i " ] " => case e o n i
+  notation:50 "ƛ " v " ⇒ " d => lam v d
+  notation:50 " μ " v " ⇒ " d => mu v d
+  notation:max "𝟘? " e " [zero⇒ " o " |succ " n " ⇒ " i " ] " => case e o n i
   infixr:min " $ " => ap
   infixl:70 " ⬝ " => ap
   prefix:80 "ι " => succ
@@ -36,7 +36,7 @@ namespace Term
   notation "𝟘" => zero
 
   example : Term := ‵"foo"
-  example : Term := 𝟘? ‵"bar" [zero: 𝟘 |succ "n" : ι 𝟘]
+  example : Term := 𝟘? ‵"bar" [zero⇒ 𝟘 |succ "n" ⇒ ι 𝟘]
 
   @[simp] def ofNat | 0 => zero | n + 1 => succ <| ofNat n
   instance : Coe ℕ Term where coe := ofNat
@@ -45,22 +45,22 @@ namespace Term
   example : Term := 1
   example : Term := 42
 
-  abbrev add : Term := μ "+" : ƛ "m" : ƛ "n" : 𝟘? ‵"m" [zero: ‵"n" |succ "m": ι (‵"+" ⬝ ‵"m" ⬝ ‵"n")]
+  abbrev add : Term := μ "+" ⇒ ƛ "m" ⇒ ƛ "n" ⇒ 𝟘? ‵"m" [zero⇒ ‵"n" |succ "m"⇒ ι (‵"+" ⬝ ‵"m" ⬝ ‵"n")]
   -- https://plfa.github.io/Lambda/#exercise-mul-recommended
-  abbrev mul : Term := μ "*" : ƛ "m" : ƛ "n" : 𝟘? ‵"m" [zero: 𝟘 |succ "m": add ⬝ ‵"n" $ ‵"*" ⬝ ‵"m" ⬝ ‵"n"]
+  abbrev mul : Term := μ "*" ⇒ ƛ "m" ⇒ ƛ "n" ⇒ 𝟘? ‵"m" [zero⇒ 𝟘 |succ "m"⇒ add ⬝ ‵"n" $ ‵"*" ⬝ ‵"m" ⬝ ‵"n"]
 
   -- Church encoding...
-  abbrev succC : Term := ƛ "n" : ι ‵"n"
-  abbrev oneC : Term := ƛ "s" : ƛ "z" : ‵"s" $ ‵"z"
-  abbrev twoC : Term := ƛ "s" : ƛ "z" : ‵"s" $ ‵"s" $ ‵"z"
-  abbrev addC : Term := ƛ "m" : ƛ "n" : ƛ "s" : ƛ "z" : ‵"m" ⬝ ‵"s" $ ‵"n" ⬝ ‵"s" ⬝ ‵"z"
+  abbrev succC : Term := ƛ "n" ⇒ ι ‵"n"
+  abbrev oneC : Term := ƛ "s" ⇒ ƛ "z" ⇒ ‵"s" $ ‵"z"
+  abbrev twoC : Term := ƛ "s" ⇒ ƛ "z" ⇒ ‵"s" $ ‵"s" $ ‵"z"
+  abbrev addC : Term := ƛ "m" ⇒ ƛ "n" ⇒ ƛ "s" ⇒ ƛ "z" ⇒ ‵"m" ⬝ ‵"s" $ ‵"n" ⬝ ‵"s" ⬝ ‵"z"
   -- https://plfa.github.io/Lambda/#exercise-mul%E1%B6%9C-practice
-  abbrev mulC : Term := ƛ "m" : ƛ "n" : ƛ "s" : ƛ "z" : ‵"m" ⬝ (‵"n" ⬝ ‵"s") ⬝ ‵"z"
+  abbrev mulC : Term := ƛ "m" ⇒ ƛ "n" ⇒ ƛ "s" ⇒ ƛ "z" ⇒ ‵"m" ⬝ (‵"n" ⬝ ‵"s") ⬝ ‵"z"
 end Term
 
 -- https://plfa.github.io/Lambda/#values
 inductive Value : Term → Type where
-| lam : Value (ƛ v : d)
+| lam : Value (ƛ v ⇒ d)
 | zero: Value 𝟘
 | succ: Value n → Value (ι n)
 deriving BEq, DecidableEq, Repr
@@ -83,31 +83,31 @@ namespace Term
   -/
   def subst : Term → Sym → Term → Term
   | ‵x, y, v => if x = y then v else ‵x
-  | ƛ x : n, y, v => if x = y then ƛ x : n else ƛ x : n.subst y v
+  | ƛ x ⇒ n, y, v => if x = y then ƛ x ⇒ n else ƛ x ⇒ n.subst y v
   | ap l m, y, v => l.subst y v $ m.subst y v
   | 𝟘, _, _ => 𝟘
   | ι n, y, v => ι (n.subst y v)
-  | 𝟘? l [zero: m |succ x: n], y, v => if x = y
-      then 𝟘? l.subst y v [zero: m.subst y v |succ x: n]
-      else 𝟘? l.subst y v [zero: m.subst y v |succ x: n.subst y v]
-  | μ x : n, y, v => if x = y then μ x : n else μ x : n.subst y v
+  | 𝟘? l [zero⇒ m |succ x⇒ n], y, v => if x = y
+      then 𝟘? l.subst y v [zero⇒ m.subst y v |succ x⇒ n]
+      else 𝟘? l.subst y v [zero⇒ m.subst y v |succ x⇒ n.subst y v]
+  | μ x⇒ n, y, v => if x = y then μ x⇒ n else μ x⇒ n.subst y v
 
   notation:90 x " [ " y " := " v " ] " => subst x y v
 
   -- https://plfa.github.io/Lambda/#examples
   example
-  : (ƛ "z" : ‵"s" ⬝ ‵"s" ⬝ ‵"z")["s" := succC]
-  = (ƛ "z" : succC ⬝ succC ⬝ ‵"z") := rfl
+  : (ƛ "z" ⇒ ‵"s" ⬝ ‵"s" ⬝ ‵"z")["s" := succC]
+  = (ƛ "z" ⇒ succC ⬝ succC ⬝ ‵"z") := rfl
 
   example : (succC ⬝ succC ⬝ ‵"z")["z" := 𝟘] = succC ⬝ succC ⬝ 𝟘 := rfl
-  example : (ƛ "x" : ‵"y")["y" := 𝟘] = (ƛ "x" : 𝟘) := rfl
-  example : (ƛ "x" : ‵"x")["x" := 𝟘] = (ƛ "x" : ‵"x") := rfl
-  example : (ƛ "y" : ‵"y")["x" := 𝟘] = (ƛ "y" : ‵"y") := rfl
+  example : (ƛ "x" ⇒ ‵"y")["y" := 𝟘] = (ƛ "x" ⇒ 𝟘) := rfl
+  example : (ƛ "x" ⇒ ‵"x")["x" := 𝟘] = (ƛ "x" ⇒ ‵"x") := rfl
+  example : (ƛ "y" ⇒ ‵"y")["x" := 𝟘] = (ƛ "y" ⇒ ‵"y") := rfl
 
   -- https://plfa.github.io/Lambda/#quiz
   example
-  : (ƛ "y" : ‵"x" $ ƛ "x" : ‵"x")["x" := 𝟘]
-  = (ƛ "y" : 𝟘 $ ƛ "x" : ‵"x")
+  : (ƛ "y" ⇒ ‵"x" $ ƛ "x" ⇒ ‵"x")["x" := 𝟘]
+  = (ƛ "y" ⇒ 𝟘 $ ƛ "x" ⇒ ‵"x")
   := rfl
 
   -- https://plfa.github.io/Lambda/#reduction
@@ -115,14 +115,14 @@ namespace Term
   `Reduce t t'` says that `t` reduces to `t'`.
   -/
   inductive Reduce : Term → Term → Type where
-  | lamβ : Value v → Reduce ((ƛ x : n) ⬝ v) (n[x := v])
+  | lamβ : Value v → Reduce ((ƛ x ⇒ n) ⬝ v) (n[x := v])
   | apξ₁ : Reduce l l' → Reduce (l ⬝ m) (l' ⬝ m)
   | apξ₂ : Value v → Reduce m m' → Reduce (v ⬝ m) (v ⬝ m')
-  | zeroβ : Reduce (𝟘? 𝟘 [zero: m |succ x : n]) m
-  | succβ : Value v → Reduce (𝟘? ι v [zero: m |succ x : n]) (n[x := v])
+  | zeroβ : Reduce (𝟘? 𝟘 [zero⇒ m |succ x ⇒ n]) m
+  | succβ : Value v → Reduce (𝟘? ι v [zero⇒ m |succ x ⇒ n]) (n[x := v])
   | succξ : Reduce m m' → Reduce (ι m) (ι m')
-  | caseξ : Reduce l l' → Reduce (𝟘? l [zero: m |succ x : n]) (𝟘? l' [zero: m |succ x : n])
-  | muβ : Reduce (μ x : m) (m[x := μ x : m])
+  | caseξ : Reduce l l' → Reduce (𝟘? l [zero⇒ m |succ x ⇒ n]) (𝟘? l' [zero⇒ m |succ x ⇒ n])
+  | muβ : Reduce (μ x⇒ m) (m[x := μ x⇒ m])
   deriving Repr
 
   infix:40 " —→ " => Reduce
@@ -130,13 +130,13 @@ end Term
 
 namespace Term.Reduce
   -- https://plfa.github.io/Lambda/#quiz-1
-  example : (ƛ "x" : ‵"x") ⬝ (ƛ "x" : ‵"x") —→ (ƛ "x" : ‵"x") := by
+  example : (ƛ "x" ⇒ ‵"x") ⬝ (ƛ "x" ⇒ ‵"x") —→ (ƛ "x" ⇒ ‵"x") := by
     apply lamβ; exact Value.lam
 
-  example : (ƛ "x" : ‵"x") ⬝ (ƛ "x" : ‵"x") ⬝ (ƛ "x" : ‵"x") —→ (ƛ "x" : ‵"x") ⬝ (ƛ "x" : ‵"x") := by
+  example : (ƛ "x" ⇒ ‵"x") ⬝ (ƛ "x" ⇒ ‵"x") ⬝ (ƛ "x" ⇒ ‵"x") —→ (ƛ "x" ⇒ ‵"x") ⬝ (ƛ "x" ⇒ ‵"x") := by
     apply apξ₁; apply lamβ; exact Value.lam
 
-  example : twoC ⬝ succC ⬝ 𝟘 —→ (ƛ "z" : succC $ succC $ ‵"z") ⬝ 𝟘 := by
+  example : twoC ⬝ succC ⬝ 𝟘 —→ (ƛ "z" ⇒ succC $ succC $ ‵"z") ⬝ 𝟘 := by
     unfold twoC; apply apξ₁; apply lamβ; exact Value.lam
 
   -- https://plfa.github.io/Lambda/#reflexive-and-transitive-closure
@@ -248,7 +248,7 @@ section examples
 
   example : twoC ⬝ succC ⬝ 𝟘 —↠ 2 := calc
     twoC ⬝ succC ⬝ 𝟘
-    _ —→ (ƛ "z" : succC $ succC $ ‵"z") ⬝ 𝟘 := by apply apξ₁; apply lamβ; exact Value.lam
+    _ —→ (ƛ "z" ⇒ succC $ succC $ ‵"z") ⬝ 𝟘 := by apply apξ₁; apply lamβ; exact Value.lam
     _ —→ (succC $ succC $ 𝟘) := by apply lamβ; exact Value.zero
     _ —→ succC ⬝ 1 := by apply apξ₂; apply Value.lam; apply lamβ; exact Value.zero
     _ —→ 2 := by apply lamβ; exact Value.ofNat 1
@@ -256,19 +256,19 @@ section examples
   -- https://plfa.github.io/Lambda/#exercise-plus-example-practice
   example : add ⬝ 1 ⬝ 1 —↠ 2 := calc
     add ⬝ 1 ⬝ 1
-    _ —→ (ƛ "m" : ƛ "n" : 𝟘? ‵"m" [zero: ‵"n" |succ "m": ι (add ⬝ ‵"m" ⬝ ‵"n")]) ⬝ 1 ⬝ 1
+    _ —→ (ƛ "m" ⇒ ƛ "n" ⇒ 𝟘? ‵"m" [zero⇒ ‵"n" |succ "m" ⇒ ι (add ⬝ ‵"m" ⬝ ‵"n")]) ⬝ 1 ⬝ 1
       := by apply apξ₁; apply apξ₁; apply muβ
-    _ —↠ (ƛ "n" : 𝟘? 1 [zero: ‵"n" |succ "m": ι (add ⬝ ‵"m" ⬝ ‵"n")]) ⬝ 1
+    _ —↠ (ƛ "n" ⇒ 𝟘? 1 [zero⇒ ‵"n" |succ "m" ⇒ ι (add ⬝ ‵"m" ⬝ ‵"n")]) ⬝ 1
       := .one <| by apply apξ₁; apply lamβ; exact Value.ofNat 1
-    _ —→ 𝟘? 1 [zero: 1 |succ "m": ι (add ⬝ ‵"m" ⬝ 1)]
+    _ —→ 𝟘? 1 [zero⇒ 1 |succ "m" ⇒ ι (add ⬝ ‵"m" ⬝ 1)]
       := lamβ <| Value.ofNat 1
     _ —→ ι (add ⬝ 𝟘 ⬝ 1)
       := succβ Value.zero
-    _ —→ ι ((ƛ "m" : ƛ "n" : 𝟘? ‵"m" [zero: ‵"n" |succ "m": ι (add ⬝ ‵"m" ⬝ ‵"n")]) ⬝ 𝟘 ⬝ 1)
+    _ —→ ι ((ƛ "m" ⇒ ƛ "n" ⇒ 𝟘? ‵"m" [zero⇒ ‵"n" |succ "m" ⇒ ι (add ⬝ ‵"m" ⬝ ‵"n")]) ⬝ 𝟘 ⬝ 1)
       := by apply succξ; apply apξ₁; apply apξ₁; apply muβ
-    _ —→ ι ((ƛ "n" : 𝟘? 𝟘 [zero: ‵"n" |succ "m": ι (add ⬝ ‵"m" ⬝ ‵"n")]) ⬝ 1)
+    _ —→ ι ((ƛ "n" ⇒ 𝟘? 𝟘 [zero⇒ ‵"n" |succ "m" ⇒ ι (add ⬝ ‵"m" ⬝ ‵"n")]) ⬝ 1)
       := by apply succξ; apply apξ₁; apply lamβ; exact V𝟘
-    _ —→ ι (𝟘? 𝟘 [zero: 1 |succ "m": ι (add ⬝ ‵"m" ⬝ 1)])
+    _ —→ ι (𝟘? 𝟘 [zero⇒ 1 |succ "m" ⇒ ι (add ⬝ ‵"m" ⬝ 1)])
       := by apply succξ; apply lamβ; exact Value.ofNat 1
     _ —→ 2 := succξ zeroβ
 end examples
@@ -342,12 +342,12 @@ namespace Context
   -/
   inductive IsTy : Context → Term → Ty → Type where
   | tyVar : Γ ∋ x ⦂ t → IsTy Γ (‵x) t
-  | tyLam : IsTy (Γ‚ x ⦂ t) n u → IsTy Γ (ƛ x : n) (t =⇒ u)
+  | tyLam : IsTy (Γ‚ x ⦂ t) n u → IsTy Γ (ƛ x ⇒ n) (t =⇒ u)
   | tyAp : IsTy Γ l (t =⇒ u) → IsTy Γ x t → IsTy Γ (l ⬝ x) u
   | tyZero : IsTy Γ 𝟘 ℕt
   | tySucc : IsTy Γ n ℕt → IsTy Γ (ι n) ℕt
-  | tyCase : IsTy Γ l ℕt → IsTy Γ m t → IsTy (Γ‚ x ⦂ ℕt) n t → IsTy Γ (𝟘? l [zero: m |succ x: n]) t
-  | tyMu : IsTy (Γ‚ x ⦂ t) m t → IsTy Γ (μ x : m) t
+  | tyCase : IsTy Γ l ℕt → IsTy Γ m t → IsTy (Γ‚ x ⦂ ℕt) n t → IsTy Γ (𝟘? l [zero⇒ m |succ x⇒ n]) t
+  | tyMu : IsTy (Γ‚ x ⦂ t) m t → IsTy Γ (μ x⇒ m) t
   deriving DecidableEq
 
   -- set_option quotPrecheck false in
@@ -376,14 +376,14 @@ namespace Context
   open Context.IsTy
 
   -- https://plfa.github.io/Lambda/#quiz-2
-  def twice_ty : Γ ⊢ (ƛ "s" : ‵"s" $ ‵"s" $ 𝟘) ⦂ ((ℕt =⇒ ℕt) =⇒ ℕt) := by
+  def twice_ty : Γ ⊢ (ƛ "s" ⇒ ‵"s" $ ‵"s" $ 𝟘) ⦂ ((ℕt =⇒ ℕt) =⇒ ℕt) := by
     apply tyLam; apply tyAp
     · trivial
     · apply tyAp
       · trivial
       · exact tyZero
 
-  def two_ty : Γ ⊢ (ƛ "s" : ‵"s" $ ‵"s" $ 𝟘) ⬝ succC ⦂ ℕt := by
+  def two_ty : Γ ⊢ (ƛ "s" ⇒ ‵"s" $ ‵"s" $ 𝟘) ⬝ succC ⦂ ℕt := by
     apply tyAp twice_ty
     · apply tyLam; apply tySucc; trivial
 
@@ -419,7 +419,7 @@ section examples
   example : ∅ ⊬ 𝟘 ⬝ 1 :=
     ⟨fun | .tyAp hl _ => by cases hl⟩
 
-  abbrev illLam := ƛ "x" : ‵"x" ⬝ ‵"x"
+  abbrev illLam := ƛ "x" ⇒ ‵"x" ⬝ ‵"x"
 
   lemma nty_illLam : ∅ ⊬ illLam :=
     ⟨fun | .tyLam (.tyAp (.tyVar hx) (.tyVar hx')) => Ty.t_to_t'_ne_t _ _ (Lookup.functional hx hx')⟩
@@ -431,7 +431,7 @@ section examples
   example : ∅‚ "y" ⦂ ℕt =⇒ ℕt‚ "x" ⦂ ℕt ⊬ ‵"x" ⬝ ‵"y" :=
     ⟨fun | .tyAp (.tyVar hx) _ => by cases hx with | s _ _ => contradiction⟩
 
-  example : ∅‚ "y" ⦂ ℕt =⇒ ℕt ⊢ ƛ "x" : ‵"y" ⬝ ‵"x" ⦂ ℕt =⇒ ℕt := by
+  example : ∅‚ "y" ⦂ ℕt =⇒ ℕt ⊢ ƛ "x" ⇒ ‵"y" ⬝ ‵"x" ⦂ ℕt =⇒ ℕt := by
     apply tyLam; apply tyAp <;> trivial
 
   example : ∅‚ "x" ⦂ t ⊬ ‵"x" ⬝ ‵"x" :=
@@ -441,7 +441,7 @@ section examples
 
   example
   : ∅‚ "x" ⦂ ℕt =⇒ ℕt‚ "y" ⦂ ℕt =⇒ ℕt
-  ⊢ ƛ "z" : (‵"x" $ ‵"y" $ ‵"z") ⦂ ℕt =⇒ ℕt
+  ⊢ ƛ "z" ⇒ (‵"x" $ ‵"y" $ ‵"z") ⦂ ℕt =⇒ ℕt
   := by
     apply tyLam; apply tyAp <;> try trivial
     · apply tyAp <;> trivial
